some fixes

BlockCacheSystem/BlockJournalCache.i.dfy
@@ -34,4 +34,38 @@ module BlockJournalCache {
   {
     exists vop :: NextStep(k, s, s', uiop, dop, vop)
   }
+
+  predicate Inv(k: Constants, s: Variables)
+  {
+    && BetreeCache.Inv(k.bc, s.bc)
+    && JournalCache.Inv(k.jc, s.jc)
+
+    && (s.jc.LoadingSuperblock? ==> s.bc.Unready?)
+    && ((s.jc.Ready? && s.jc.isFrozen) <==>
+        (s.bc.Ready? && s.bc.frozenIndirectionTable.Some?))
+    && (s.jc.Ready? && s.jc.frozenLoc.Some? ==>
+      && s.bc.Ready?
+      && s.bc.frozenIndirectionTableLoc == s.jc.frozenLoc
+      && s.bc.outstandingIndirectionTableWrite.None?
+    )
+  }
+
+  lemma InitImpliesInv(k: Constants, s: Variables)
+  requires Init(k, s)
+  ensures Inv(k, s)
+  {
+    BetreeCache.InitImpliesInv(k.bc, s.bc);
+    JournalCache.InitImpliesInv(k.jc, s.jc);
+  }
+
+  lemma NextPreservesInv(k: Constants, s: Variables, s': Variables, uiop: UI.Op, dop: D.DiskOp)
+  requires Inv(k, s)
+  requires Next(k, s, s', uiop, dop)
+  ensures Inv(k, s')
+  {
+    var vop :| NextStep(k, s, s', uiop, dop, vop);
+    BetreeCache.NextPreservesInv(k.bc, s.bc, s'.bc, dop.bdop, vop);
+    JournalCache.NextPreservesInv(k.jc, s.jc, s'.jc, dop.jdop, vop);
+  }
+
 }
