Impl/MainHandlers.i.dfy
@@ -4,31 +4,37 @@ include "CoordinationImpl.i.dfy"
 include "HandleReadResponseImpl.i.dfy"
 include "HandleWriteResponseImpl.i.dfy"
 include "Mkfs.i.dfy"
+include "CoordinationModel.i.dfy"
+include "../ByteBlockCacheSystem/ByteSystem_Refines_ThreeStateVersionedMap.i.dfy"
 
 //
 // Implements the application-API-handler obligations laid out by Main.s.dfy. TODO rename in a way that emphasizes that this is a module-refinement of the abstract Main that satisfies its obligations.
 //
 
 module {:extern} MainHandlers refines Main { 
+  import DOM = DiskOpModel
   import SM = StateModel
   import SI = StateImpl
-  import CoordinationModel
   import CoordinationImpl
   import HandleReadResponseImpl
   import HandleReadResponseModel
   import HandleWriteResponseImpl
   import HandleWriteResponseModel
+  import CoordinationModel
   import FullImpl
-  import opened DiskOpImpl
-  import opened MainDiskIOHandler
   import MkfsImpl
   import MkfsModel
 
+  import BlockJournalCache
   import BBC = BetreeCache
   import BC = BlockCache
+  import JC = JournalCache
   import ADM = ByteSystem
 
-  import System_Ref = ByteBetreeBlockCacheSystem_Refines_ThreeStateVersionedMap
+  import opened DiskOpImpl
+  import opened InterpretationDiskOps
+
+  import System_Ref = ByteSystem_Refines_ThreeStateVersionedMap
 
   type Constants = ImplConstants
   type Variables = FullImpl.Full
@@ -42,22 +48,26 @@ module {:extern} MainHandlers refines Main {
     && hs.s.Inv(k)
   }
 
-  function Ik(k: Constants) : ADM.M.Constants { BC.Constants() }
+  function Ik(k: Constants) : ADM.M.Constants {
+    BlockJournalCache.Constants(BC.Constants(), JC.Constants())
+  }
   function I(k: Constants, hs: HeapState) : ADM.M.Variables {
     SM.IVars(hs.s.I())
   }
 
   method InitState() returns (k: Constants, hs: HeapState)
+    // conditions inherited:
+    //ensures Inv(k, hs)
+    //ensures ADM.M.Init(Ik(k), I(k, hs))
   {
-    k := BC.Constants();
-    var s := new Variables();
+    var s := new Variables(k);
     hs := new HeapState(s, {});
-    hs.Repr := s.Repr() + {s};
+    hs.Repr := s.Repr + {s};
     assert Inv(k, hs);
-    BBC.InitImpliesInv(Ik(k), I(k, hs));
+    BlockJournalCache.InitImpliesInv(Ik(k), I(k, hs));
   }
 
-  lemma ioAndHsNotInReadSet(s: Full, io: DiskIOHandler, hs: HeapState)
+  lemma ioAndHsNotInReadSet(s: Variables, io: DiskIOHandler, hs: HeapState)
   requires s.W()
   ensures io !in s.Repr
   ensures hs !in s.Repr
@@ -71,29 +81,38 @@ module {:extern} MainHandlers refines Main {
   {
     var s := hs.s;
     ioAndHsNotInReadSet(s, io, hs);
-    CoordinatorModel.pushSyncCorrect(SI.Ic(k), s.I());
-    var id1 := CoordinatorImpl.pushSync(k, s);
+    var id1 := CoordinationImpl.pushSync(k, s);
+
+    CoordinationModel.pushSyncCorrect(Ic(k), old(s.I()));
+
+    //assert ADM.M.Next(DOM.Ik(Ic(k)), SM.IVars(old(s.I())), SM.IVars(s.I()),
+    //   if id1 == 0 then UI.NoOp else UI.PushSyncOp(id1 as int),
+    //   D.NoDiskOp);
+
     ioAndHsNotInReadSet(s, io, hs);
     id := id1;
     ghost var uiop := if id == 0 then UI.NoOp else UI.PushSyncOp(id as int);
-    BBC.NextPreservesInv(k, SM.IVars(old(s.I())), SM.IVars(s.I()), uiop, ADM.M.IDiskOp(io.diskOp()));
-    hs.Repr := s.Repr() + {s};
+    BlockJournalCache.NextPreservesInv(DOM.Ik(Ic(k)), SM.IVars(old(s.I())), SM.IVars(s.I()), uiop, IDiskOp(io.diskOp()));
+    hs.Repr := s.Repr + {s};
+    //assert SM.Inv(Ic(k), hs.s.I());
+    //assert hs.s.Inv(k);
+    //assert Inv(k, hs);
     assert ADM.M.Next(Ik(k), old(I(k, hs)), I(k, hs), uiop, io.diskOp()); // observe
   }
 
-  method handlePopSync(k: Constants, hs: HeapState, io: DiskIOHandler, id: uint64)
+  method handlePopSync(k: Constants, hs: HeapState, io: DiskIOHandler, id: uint64, graphSync: bool)
   returns (wait: bool, success: bool)
   {
     var s := hs.s;
     ioAndHsNotInReadSet(s, io, hs);
-    var w, succ := CoordinatorImpl.popSync(k, s, io, id);
-    CoordinatorModel.popSyncCorrect(SI.Ic(k), old(s.I()), old(SI.IIO(io)), id, s.I(), succ, SI.IIO(io));
+    var succ, w := CoordinationImpl.popSync(k, s, io, id, graphSync);
+    CoordinationModel.popSyncCorrect(Ic(k), old(s.I()), old(IIO(io)), id, graphSync, s.I(), IIO(io), succ);
     ioAndHsNotInReadSet(s, io, hs);
     success := succ;
     wait := w;
     ghost var uiop := if succ then UI.PopSyncOp(id as int) else UI.NoOp;
-    BBC.NextPreservesInv(k, SM.IVars(old(s.I())), SM.IVars(s.I()), uiop, ADM.M.IDiskOp(io.diskOp()));
-    hs.Repr := s.Repr() + {s};
+    BlockJournalCache.NextPreservesInv(DOM.Ik(Ic(k)), SM.IVars(old(s.I())), SM.IVars(s.I()), uiop, IDiskOp(io.diskOp()));
+    hs.Repr := s.Repr + {s};
     assert ADM.M.Next(Ik(k), old(I(k, hs)), I(k, hs), // observe
         uiop,
         io.diskOp());
@@ -104,12 +123,12 @@ module {:extern} MainHandlers refines Main {
   {
     var s := hs.s;
     ioAndHsNotInReadSet(s, io, hs);
-    var value := CoordinatorImpl.query(k, s, io, key);
-    CoordinatorModel.queryCorrect(SI.Ic(k), old(s.I()), old(SI.IIO(io)), key, s.I(), value, SI.IIO(io));
+    var value := CoordinationImpl.query(k, s, io, key);
+    CoordinationModel.queryCorrect(Ic(k), old(s.I()), old(IIO(io)), key, s.I(), value, IIO(io));
     ioAndHsNotInReadSet(s, io, hs);
     ghost var uiop := if value.Some? then UI.GetOp(key, value.value) else UI.NoOp;
-    BBC.NextPreservesInv(k, SM.IVars(old(s.I())), SM.IVars(s.I()), uiop, ADM.M.IDiskOp(io.diskOp()));
-    hs.Repr := s.Repr() + {s};
+    BlockJournalCache.NextPreservesInv(DOM.Ik(Ic(k)), SM.IVars(old(s.I())), SM.IVars(s.I()), uiop, IDiskOp(io.diskOp()));
+    hs.Repr := s.Repr + {s};
     v := value;
     assert ADM.M.Next(Ik(k), old(I(k, hs)), I(k, hs), // observe
         if v.Some? then UI.GetOp(key, v.value) else UI.NoOp,
@@ -121,12 +140,12 @@ module {:extern} MainHandlers refines Main {
   {
     var s := hs.s;
     ioAndHsNotInReadSet(s, io, hs);
-    var succ := CoordinatorImpl.insert(k, s, io, key, value);
-    CoordinatorModel.insertCorrect(SI.Ic(k), old(s.I()), old(SI.IIO(io)), key, value, s.I(), succ, SI.IIO(io));
+    var succ := CoordinationImpl.insert(k, s, io, key, value);
+    CoordinationModel.insertCorrect(Ic(k), old(s.I()), old(IIO(io)), key, value, s.I(), succ, IIO(io));
     ioAndHsNotInReadSet(s, io, hs);
     ghost var uiop := if succ then UI.PutOp(key, value) else UI.NoOp;
-    BBC.NextPreservesInv(k, SM.IVars(old(s.I())), SM.IVars(s.I()), uiop, ADM.M.IDiskOp(io.diskOp()));
-    hs.Repr := s.Repr() + {s};
+    BlockJournalCache.NextPreservesInv(DOM.Ik(Ic(k)), SM.IVars(old(s.I())), SM.IVars(s.I()), uiop, IDiskOp(io.diskOp()));
+    hs.Repr := s.Repr + {s};
     success := succ;
     assert ADM.M.Next(Ik(k), old(I(k, hs)), I(k, hs), // observe
         if success then UI.PutOp(key, value) else UI.NoOp,
@@ -138,13 +157,13 @@ module {:extern} MainHandlers refines Main {
   {
     var s := hs.s;
     ioAndHsNotInReadSet(s, io, hs);
-    var value := CoordinatorImpl.doSucc(k, s, io, start, maxToFind);
-    CoordinatorModel.doSuccCorrect(SI.Ic(k), old(s.I()), old(SI.IIO(io)), start, maxToFind as int);
+    var value := CoordinationImpl.succ(k, s, io, start, maxToFind);
+    CoordinationModel.succCorrect(Ic(k), old(s.I()), old(IIO(io)), start, maxToFind as int, s.I(), value, IIO(io));
     ioAndHsNotInReadSet(s, io, hs);
     ghost var uiop := 
       if value.Some? then UI.SuccOp(start, value.value.results, value.value.end) else UI.NoOp;
-    BBC.NextPreservesInv(k, SM.IVars(old(s.I())), SM.IVars(s.I()), uiop, ADM.M.IDiskOp(io.diskOp()));
-    hs.Repr := s.Repr() + {s};
+    BlockJournalCache.NextPreservesInv(DOM.Ik(Ic(k)), SM.IVars(old(s.I())), SM.IVars(s.I()), uiop, IDiskOp(io.diskOp()));
+    hs.Repr := s.Repr + {s};
     res := value;
     assert ADM.M.Next(Ik(k), old(I(k, hs)), I(k, hs), // observe
         uiop,
@@ -156,11 +175,11 @@ module {:extern} MainHandlers refines Main {
     var s := hs.s;
     ioAndHsNotInReadSet(s, io, hs);
     HandleReadResponseImpl.readResponse(k, s, io);
-    HandleReadResponseModel.readResponseCorrect(SI.Ic(k), old(s.I()), old(SI.IIO(io)));
+    HandleReadResponseModel.readResponseCorrect(Ic(k), old(s.I()), old(IIO(io)));
     ioAndHsNotInReadSet(s, io, hs);
     ghost var uiop := UI.NoOp;
-    BBC.NextPreservesInv(k, SM.IVars(old(s.I())), SM.IVars(s.I()), uiop, ADM.M.IDiskOp(io.diskOp()));
-    hs.Repr := s.Repr() + {s};
+    BlockJournalCache.NextPreservesInv(DOM.Ik(Ic(k)), SM.IVars(old(s.I())), SM.IVars(s.I()), uiop, IDiskOp(io.diskOp()));
+    hs.Repr := s.Repr + {s};
     assert ADM.M.Next(Ik(k), old(I(k, hs)), I(k, hs), UI.NoOp, io.diskOp()); // observe
   }
 
@@ -169,11 +188,11 @@ module {:extern} MainHandlers refines Main {
     var s := hs.s;
     ioAndHsNotInReadSet(s, io, hs);
     HandleWriteResponseImpl.writeResponse(k, s, io);
-    HandleWriteResponseModel.writeResponseCorrect(SI.Ic(k), old(s.I()), old(SI.IIO(io)));
+    HandleWriteResponseModel.writeResponseCorrect(Ic(k), old(s.I()), old(IIO(io)));
     ioAndHsNotInReadSet(s, io, hs);
     ghost var uiop := UI.NoOp;
-    BBC.NextPreservesInv(k, SM.IVars(old(s.I())), SM.IVars(s.I()), uiop, ADM.M.IDiskOp(io.diskOp()));
-    hs.Repr := s.Repr() + {s};
+    BlockJournalCache.NextPreservesInv(DOM.Ik(Ic(k)), SM.IVars(old(s.I())), SM.IVars(s.I()), uiop, IDiskOp(io.diskOp()));
+    hs.Repr := s.Repr + {s};
     assert ADM.M.Next(Ik(k), old(I(k, hs)), I(k, hs), UI.NoOp, io.diskOp()); // observe
   }
 
